<?xml version="1.0" encoding="UTF-8"?>
<rdf:RDF
   xmlns:base="http://www.ngi.ontochain/ontologies/oc-found.owl#"
   xmlns:oasis="http://www.dmi.unict.it/oasis.owl#"
   xmlns:owl="http://www.w3.org/2002/07/owl#"
   xmlns:rdf="http://www.w3.org/1999/02/22-rdf-syntax-ns#"
   xmlns:rdfs="http://www.w3.org/2000/01/rdf-schema#"
>
  <rdf:Description rdf:about="http://www.ngi.ontochain/ontologies/oc-found.owl#hasQualityValuationResult">
    <rdf:type rdf:resource="http://www.w3.org/2002/07/owl#ObjectProperty"/>
    <rdfs:domain rdf:resource="http://www.ngi.ontochain/ontologies/oc-found.owl#QualityValuationActivity"/>
    <rdfs:subPropertyOf rdf:resource="http://www.dmi.unict.it/oasis.owl#hasCompositeValue"/>
    <rdfs:comment xml:lang="en">This property connects a quality valuation activity (i.e., instance of QualityValuationActivity) to quality valuation result computed</rdfs:comment>
    <rdfs:range rdf:resource="http://www.ngi.ontochain/ontologies/oc-found.owl#QualityValuationResult"/>
  </rdf:Description>
  <rdf:Description rdf:about="http://www.ngi.ontochain/ontologies/oc-found.owl#SupplyChainActivity">
    <rdfs:subClassOf rdf:resource="http://www.ngi.ontochain/ontologies/oc-found.owl#SupplyChainThing"/>
    <rdf:type rdf:resource="http://www.w3.org/2002/07/owl#Class"/>
    <rdfs:comment xml:lang="en">This class describes an activity concerning the supply chain of resources</rdfs:comment>
  </rdf:Description>
  <rdf:Description rdf:about="http://www.ngi.ontochain/ontologies/oc-found.owl#hasSupplyChainActivity">
    <rdfs:subPropertyOf rdf:resource="http://www.dmi.unict.it/oasis.owl#encompassesActivity"/>
    <rdfs:comment xml:lang="en">This property connects a supply chain management activity to its internal activities</rdfs:comment>
    <rdf:type rdf:resource="http://www.w3.org/2002/07/owl#ObjectProperty"/>
    <rdfs:domain rdf:resource="http://www.ngi.ontochain/ontologies/oc-found.owl#SupplyChainManagement"/>
    <rdfs:range rdf:resource="http://www.ngi.ontochain/ontologies/oc-found.owl#SupplyChainActivity"/>
  </rdf:Description>
  <rdf:Description rdf:about="http://www.ngi.ontochain/ontologies/oc-found.owl#ValuerTemplateGoal">
    <oasis:consistsOfTaskDescription rdf:resource="http://www.ngi.ontochain/ontologies/oc-found.owl#ValuerTemplateTask"/>
    <rdf:type rdf:resource="http://www.dmi.unict.it/oasis.owl#GoalDescription"/>
  </rdf:Description>
  <rdf:Description rdf:about="http://www.ngi.ontochain/ontologies/oc-found.owl#ValuerTemplateTask">
    <oasis:hasTaskOutputParameterTemplate rdf:resource="http://www.ngi.ontochain/ontologies/oc-found.owl#ValuerTemplateTaskOutput1"/>
    <rdf:type rdf:resource="http://www.dmi.unict.it/oasis.owl#TaskDescription"/>
    <oasis:hasTaskInputParameterTemplate rdf:resource="http://www.ngi.ontochain/ontologies/oc-found.owl#ValuerTemplateTaskInput1"/>
    <oasis:hasTaskOperator rdf:resource="http://www.ngi.ontochain/ontologies/oc-found.owl#ValuerTemplateTaskOperator"/>
    <oasis:hasTaskObjectTemplate rdf:resource="http://www.ngi.ontochain/ontologies/oc-found.owl#ValuerTemplateTaskObject"/>
    <oasis:hasTaskOperatorArgument rdf:resource="http://www.ngi.ontochain/ontologies/oc-found.owl#ValuerTemplateTaskOperatorArgument"/>
  </rdf:Description>
  <rdf:Description rdf:about="http://www.ngi.ontochain/ontologies/oc-found.owl#SupplyChainReleaseActivity">
    <rdfs:comment xml:lang="en">This class describes the release activity  of resources involved in some supply chains.</rdfs:comment>
    <rdfs:subClassOf rdf:resource="http://www.ngi.ontochain/ontologies/oc-found.owl#SupplyChainActivity"/>
    <rdf:type rdf:resource="http://www.w3.org/2002/07/owl#Class"/>
  </rdf:Description>
  <rdf:Description rdf:about="http://www.dmi.unict.it/oasis.owl#hasTaskInputParameterTemplate">
    <rdf:type rdf:resource="http://www.w3.org/2002/07/owl#ObjectProperty"/>
  </rdf:Description>
  <rdf:Description rdf:about="http://www.ngi.ontochain/ontologies/oc-found.owl#performsQualityValuation">
    <rdf:type rdf:resource="http://www.w3.org/2002/07/owl#ObjectProperty"/>
    <rdfs:domain rdf:resource="http://www.ngi.ontochain/ontologies/oc-found.owl#QualityValuerAgent"/>
    <rdfs:comment xml:lang="en">This property connects a valuer agent (i.e., instance of QualityValuerAgent) to the performed quality valuation activity (i.e., instance of QualityValuationActivity)</rdfs:comment>
    <rdfs:subPropertyOf rdf:resource="http://www.dmi.unict.it/oasis.owl#isRelatedWithActivity"/>
    <rdfs:subPropertyOf rdf:resource="http://www.dmi.unict.it/oasis.owl#performs"/>
    <rdfs:range rdf:resource="http://www.ngi.ontochain/ontologies/oc-found.owl#QualityValuationActivity"/>
  </rdf:Description>
  <rdf:Description rdf:about="http://www.ngi.ontochain/ontologies/oc-found.owl#ValuerTemplateTaskInput1">
    <rdf:type rdf:resource="http://www.dmi.unict.it/oasis.owl#TaskInputParameterTemplate"/>
    <oasis:refersAsNewTo rdf:resource="http://www.ngi.ontochain/ontologies/oc-found.owl#objectAsset"/>
  </rdf:Description>
  <rdf:Description rdf:about="http://www.ngi.ontochain/ontologies/oc-found.owl#ValuerTemplateTaskOperator">
    <oasis:refersExactlyTo rdf:resource="http://www.dmi.unict.it/oasis-abox.owl#perform"/>
    <rdf:type rdf:resource="http://www.dmi.unict.it/oasis.owl#TaskOperator"/>
  </rdf:Description>
  <rdf:Description rdf:about="http://www.ngi.ontochain/ontologies/oc-found.owl#supplyChainActivityImplementedBy">
    <rdf:type rdf:resource="http://www.w3.org/2002/07/owl#ObjectProperty"/>
    <rdfs:domain rdf:resource="http://www.ngi.ontochain/ontologies/oc-found.owl#SupplyChainActivity"/>
    <rdfs:subPropertyOf rdf:resource="http://www.dmi.unict.it/oasis.owl#implementedBy"/>
    <rdfs:range rdf:resource="http://www.dmi.unict.it/oasis.owl#Behavior"/>
  </rdf:Description>
  <rdf:Description rdf:about="http://www.ngi.ontochain/ontologies/oc-found.owl#ValuerTemplateTaskOutput1">
    <oasis:refersAsNewTo rdf:resource="http://www.ngi.ontochain/ontologies/oc-found.owl#valuationResult"/>
    <rdf:type rdf:resource="http://www.dmi.unict.it/oasis.owl#TaskOutputParameterTemplate"/>
  </rdf:Description>
  <rdf:Description rdf:about="http://www.ngi.ontochain/ontologies/oc-found.owl#SupplyChainThing">
    <rdfs:subClassOf rdf:resource="http://www.dmi.unict.it/oasis.owl#Activity"/>
    <rdfs:comment xml:lang="en">This class  encompasses all the classes concerning the supply chain environment</rdfs:comment>
    <rdf:type rdf:resource="http://www.w3.org/2002/07/owl#Class"/>
  </rdf:Description>
  <rdf:Description rdf:about="http://www.ngi.ontochain/ontologies/oc-found.owl#QualityValuationResult">
    <rdf:type rdf:resource="http://www.w3.org/2002/07/owl#Class"/>
    <rdfs:subClassOf rdf:resource="http://www.dmi.unict.it/oasis.owl#CompositeValue"/>
    <rdfs:comment xml:lang="en">This class describes the output of a quality valuation performed by a quality valuer agent, i.e., instance of QualityValuerAgent</rdfs:comment>
  </rdf:Description>
  <rdf:Description rdf:about="http://www.ngi.ontochain/ontologies/oc-found.owl#hasSupplyChainManagement">
    <rdf:type rdf:resource="http://www.w3.org/2002/07/owl#ObjectProperty"/>
    <rdfs:range rdf:resource="http://www.ngi.ontochain/ontologies/oc-found.owl#SupplyChainManagement"/>
    <rdfs:comment xml:lang="en">This property connects a resource to its supply chain management activity</rdfs:comment>
    <rdfs:subPropertyOf rdf:resource="http://www.dmi.unict.it/oasis.owl#isRelatedWithActivity"/>
  </rdf:Description>
  <rdf:Description rdf:about="http://www.ngi.ontochain/ontologies/oc-found.owl#SupplyChainDeliveryActivity">
    <rdfs:subClassOf rdf:resource="http://www.ngi.ontochain/ontologies/oc-found.owl#SupplyChainActivity"/>
    <rdf:type rdf:resource="http://www.w3.org/2002/07/owl#Class"/>
    <rdfs:comment xml:lang="en">This class describes the delivery activity  of resources involved in some supply chains.</rdfs:comment>
  </rdf:Description>
  <rdf:Description rdf:about="http://www.ngi.ontochain/ontologies/oc-found.owl#SupplyChainPaymentActivity">
    <rdfs:comment xml:lang="en">This class describes the payment activity  of resources involved in some supply chains.</rdfs:comment>
    <rdf:type rdf:resource="http://www.w3.org/2002/07/owl#Class"/>
    <rdfs:subClassOf rdf:resource="http://www.ngi.ontochain/ontologies/oc-found.owl#SupplyChainActivity"/>
  </rdf:Description>
  <rdf:Description rdf:about="http://www.ngi.ontochain/ontologies/oc-found.owl#hasDigitalIdentity">
    <rdf:type rdf:resource="http://www.w3.org/2002/07/owl#ObjectProperty"/>
    <rdfs:comment xml:lang="en">This property connects agents to their digital identities, i.e., instance of DigitalIdentity</rdfs:comment>
    <rdfs:range rdf:resource="http://www.ngi.ontochain/ontologies/oc-found.owl#DigitalIdentity"/>
    <rdfs:domain rdf:resource="http://www.dmi.unict.it/oasis.owl#Agent"/>
    <rdfs:subPropertyOf rdf:resource="http://www.dmi.unict.it/oasis.owl#owns"/>
  </rdf:Description>
  <rdf:Description rdf:about="http://www.ngi.ontochain/ontologies/oc-found.owl#DigitalIdentity">
    <rdf:type rdf:resource="http://www.w3.org/2002/07/owl#Class"/>
    <rdfs:subClassOf rdf:resource="http://www.dmi.unict.it/oasis.owl#DescriptionObject"/>
    <rdfs:comment xml:lang="en">This class describes the digital identities associated with legal entities or agents</rdfs:comment>
  </rdf:Description>
  <rdf:Description rdf:about="http://www.dmi.unict.it/oasis.owl#hasTaskOutputParameterTemplate">
    <rdf:type rdf:resource="http://www.w3.org/2002/07/owl#ObjectProperty"/>
  </rdf:Description>
  <rdf:Description rdf:about="http://www.ngi.ontochain/ontologies/oc-found.owl#valuationResult">
    <rdf:type rdf:resource="http://www.dmi.unict.it/oasis.owl#QualityValuationResult"/>
  </rdf:Description>
  <rdf:Description rdf:about="http://www.ngi.ontochain/ontologies/oc-found.owl#QualityValuerAgent">
    <rdfs:subClassOf rdf:resource="http://www.dmi.unict.it/oasis.owl#Agent"/>
    <rdfs:comment xml:lang="en">This class describes a quality valuer agent, i.e., an agent performing quality valuations on resources of supply chain activities.</rdfs:comment>
    <rdf:type rdf:resource="http://www.w3.org/2002/07/owl#Class"/>
  </rdf:Description>
  <rdf:Description rdf:about="http://www.dmi.unict.it/oasis.owl#consistsOfTaskDescription">
    <rdf:type rdf:resource="http://www.w3.org/2002/07/owl#ObjectProperty"/>
  </rdf:Description>
  <rdf:Description rdf:about="http://www.dmi.unict.it/oasis.owl#refersAsNewTo">
    <rdf:type rdf:resource="http://www.w3.org/2002/07/owl#ObjectProperty"/>
  </rdf:Description>
  <rdf:Description rdf:about="http://www.ngi.ontochain/ontologies/oc-found.owl#SupplyChainManagement">
    <rdfs:subClassOf rdf:resource="http://www.ngi.ontochain/ontologies/oc-found.owl#SupplyChainThing"/>
    <rdf:type rdf:resource="http://www.w3.org/2002/07/owl#Class"/>
    <rdfs:comment xml:lang="en">This class describes the management activity concerning supply chain of resources</rdfs:comment>
  </rdf:Description>
  <rdf:Description rdf:about="http://www.dmi.unict.it/oasis.owl#consistsOfGoalDescription">
    <rdf:type rdf:resource="http://www.w3.org/2002/07/owl#ObjectProperty"/>
  </rdf:Description>
  <rdf:Description rdf:about="http://www.ngi.ontochain/ontologies/oc-found.owl#objectAsset">
    <rdf:type rdf:resource="http://www.dmi.unict.it/oasis.owl#Asset"/>
  </rdf:Description>
  <rdf:Description rdf:about="http://www.ngi.ontochain/ontologies/oc-found.owl#valuationActivityObject">
    <base:hasQualityValuationResult rdf:resource="http://www.ngi.ontochain/ontologies/oc-found.owl#valuationResult"/>
    <base:qualityValuationPerformedOn rdf:resource="http://www.ngi.ontochain/ontologies/oc-found.owl#objectAsset"/>
    <rdf:type rdf:resource="http://www.ngi.ontochain/ontologies/oc-found.owl#QualityValuationActivity"/>
  </rdf:Description>
  <rdf:Description rdf:about="http://www.dmi.unict.it/oasis.owl#hasBehavior">
    <rdf:type rdf:resource="http://www.w3.org/2002/07/owl#ObjectProperty"/>
  </rdf:Description>
  <rdf:Description rdf:about="http://www.ngi.ontochain/ontologies/oc-found.owl">
    <rdf:type rdf:resource="http://www.w3.org/2002/07/owl#Ontology"/>
    <owl:imports rdf:resource="http://www.dmi.unict.it/oasis.owl"/>
    <owl:imports rdf:resource="http://www.dmi.unict.it/oasis-abox.owl"/>
  </rdf:Description>
  <rdf:Description rdf:about="http://www.ngi.ontochain/ontologies/oc-found.owl#qualityValuationPerformedOn">
    <rdfs:comment xml:lang="en">This property connects a quality valuation activity (i.e., instance of QualityValuationActivity) to the resource for which the quality valuation has been performed</rdfs:comment>
    <rdf:type rdf:resource="http://www.w3.org/2002/07/owl#ObjectProperty"/>
    <rdfs:domain rdf:resource="http://www.ngi.ontochain/ontologies/oc-found.owl#QualityValuationActivity"/>
    <rdfs:subPropertyOf rdf:resource="http://www.dmi.unict.it/oasis.owl#involves"/>
  </rdf:Description>
  <rdf:Description rdf:about="http://www.ngi.ontochain/ontologies/oc-found.owl#QualityValuationActivity">
    <rdfs:comment xml:lang="en">This class describes a quality valuation activity performed by some quality valuer agents (i.e., instance of QualityValuerAgent)</rdfs:comment>
    <rdfs:subClassOf rdf:resource="http://www.dmi.unict.it/oasis.owl#Activity"/>
    <rdf:type rdf:resource="http://www.w3.org/2002/07/owl#Class"/>
  </rdf:Description>
  <rdf:Description rdf:about="http://www.ngi.ontochain/ontologies/oc-found.owl#ValuerTemplateTaskOperatorArgument">
    <oasis:refersExactlyTo rdf:resource="http://www.dmi.unict.it/oasis-abox.owl#quality_evaluation"/>
    <rdf:type rdf:resource="http://www.dmi.unict.it/oasis.owl#TaskOperatorArgument"/>
  </rdf:Description>
  <rdf:Description rdf:about="http://www.ngi.ontochain/ontologies/oc-found.owl#ValuerAgentBehaviorTemplate">
    <rdf:type rdf:resource="http://www.dmi.unict.it/oasis.owl#AgentBehaviorTemplate"/>
    <oasis:hasBehavior rdf:resource="http://www.ngi.ontochain/ontologies/oc-found.owl#ValuerTemplateBehavior"/>
  </rdf:Description>
  <rdf:Description rdf:about="http://www.ngi.ontochain/ontologies/oc-found.owl#SupplyChainProofWorkActivity">
    <rdf:type rdf:resource="http://www.w3.org/2002/07/owl#Class"/>
    <rdfs:subClassOf rdf:resource="http://www.ngi.ontochain/ontologies/oc-found.owl#SupplyChainActivity"/>
  </rdf:Description>
  <rdf:Description rdf:about="http://www.ngi.ontochain/ontologies/oc-found.owl#ValuerTemplateTaskObject">
    <oasis:refersAsNewTo rdf:resource="http://www.ngi.ontochain/ontologies/oc-found.owl#valuationActivityObject"/>
    <rdf:type rdf:resource="http://www.dmi.unict.it/oasis.owl#TaskObjectTemplate"/>
  </rdf:Description>
  <rdf:Description rdf:about="http://www.ngi.ontochain/ontologies/oc-found.owl#ValuerTemplateBehavior">
    <rdf:type rdf:resource="http://www.dmi.unict.it/oasis.owl#Behavior"/>
    <oasis:consistsOfGoalDescription rdf:resource="http://www.ngi.ontochain/ontologies/oc-found.owl#ValuerTemplateGoal"/>
  </rdf:Description>
  <rdf:Description rdf:about="http://www.dmi.unict.it/oasis.owl#hasTaskOperatorArgument">
    <rdf:type rdf:resource="http://www.w3.org/2002/07/owl#ObjectProperty"/>
  </rdf:Description>
  <rdf:Description rdf:about="http://www.dmi.unict.it/oasis.owl#hasTaskObjectTemplate">
    <rdf:type rdf:resource="http://www.w3.org/2002/07/owl#ObjectProperty"/>
  </rdf:Description>
  <rdf:Description rdf:about="http://www.ngi.ontochain/ontologies/oc-found.owl#LegalEntity">
    <rdfs:subClassOf rdf:resource="http://www.dmi.unict.it/oasis.owl#Agent"/>
    <rdf:type rdf:resource="http://www.w3.org/2002/07/owl#Class"/>
    <rdfs:comment xml:lang="en">This class describes legal entities such as companies, people, societies</rdfs:comment>
  </rdf:Description>
  <rdf:Description rdf:about="http://www.dmi.unict.it/oasis-abox.owl#perform">
    <rdf:type rdf:resource="http://www.dmi.unict.it/oasis.owl#Action"/>
  </rdf:Description>
  <rdf:Description rdf:about="http://www.dmi.unict.it/oasis.owl#refersExactlyTo">
    <rdf:type rdf:resource="http://www.w3.org/2002/07/owl#ObjectProperty"/>
  </rdf:Description>
  <rdf:Description rdf:about="http://www.dmi.unict.it/oasis-abox.owl#quality_evaluation">
    <rdf:type rdf:resource="http://www.dmi.unict.it/oasis.owl#DescriptionObject"/>
  </rdf:Description>
  <rdf:Description rdf:about="http://www.dmi.unict.it/oasis.owl#hasTaskOperator">
    <rdf:type rdf:resource="http://www.w3.org/2002/07/owl#ObjectProperty"/>
  </rdf:Description>
</rdf:RDF>
